example

minuska/src/example_lang_driver.ml
@@ -4,6 +4,8 @@ let usage_msg = "example_langdriver [-verbose] <number>"
 
 let verbose = ref false
 
+let depth = ref 10
+
 let number = ref 0
 
 
@@ -11,7 +13,9 @@ let anon_fun mynum =
   number := int_of_string mynum
 
 let speclist =
-  [("-verbose", Arg.Set verbose, "Output debug information")
+  [
+    ("-verbose", Arg.Set verbose, "Output debug information");
+    ("-depth", Arg.Set_int depth, "Maximal execution depth")
   ]
 
 let () =
@@ -19,5 +23,9 @@ let () =
   (* Main functionality here *)
   print_string "Hello world!\n";
   print_string (string_of_int !number);
-  let result = interp_number !number in
-  result
+  print_string (string_of_int !depth);
+  let result = ExampleLang.Coq_example_1.interp_loop_number !depth !number in
+  match result with
+  | None -> print_string "None"
+  | Some x -> print_string "Some"; print_string (string_of_int x)
+  
